Project finally documented

coq_files/src/Theorems/theorems.v
@@ -1,10 +1,18 @@
-(* Imports: *) 
-Require Import Hbt.Lemmas.Ordered.ordered_main.
+(* ********** theorems.v ********** *)
 
+(** The [theorems] library contains the specifications for the lookup and insert 
+functions on AVL trees, and the theorems which show that our implementation of these
+operations (see the [hbt] library) meet the specifications *)
 
-(* ***** Section 1: Specification and associated theorems for lookup ***** *)
+Require Import Hbt.Lemmas.Ordered.Main.ordered_main.
 
-(* The specification *)
+(* ********** *)
+
+(** * Lookup *)
+
+(** Defining the specification for a lookup function looking for some value <<x>>: 
+- if the tree is a leaf, then the function should always return a [false] value
+- if the tree is a node with a left sub-tree <<hbt1>>, a payload <<e>>, and a right sub-tree <<hbt2>>, then the function should compare <<x>> and <<e>>, returning true if the equality holds, checking <<hbt1>> if <<x>> is less than <<e>>, checking <<hbt2>> otherwise *)
 Definition specification_of_occurs_hbt
            (A : Type)
            (compare : A -> A -> element_comparison)
@@ -13,98 +21,62 @@ Definition specification_of_occurs_hbt
                -> A'
                -> heightened_binary_tree A'
                -> bool) :=
-  forall (e : A)
-         (h : nat)
-         (bt : binary_tree A),
-  exists (occ_bt : forall (A' : Type),
-             (A' -> A' -> element_comparison) -> A' -> binary_tree A' -> bool),
-    occ_hbt A compare e (HNode A h bt) = occ_bt A compare e bt.
+  forall (hbt : heightened_binary_tree A)
+         (x : A),
+    specification_of_compare_defining_total_order A compare -> 
+    (hbt = (HNode A 0 (Leaf A)) -> occ_hbt A compare x hbt = false)
+    /\
+    (forall (hbt1 hbt2 : heightened_binary_tree A)
+            (h_hbt : nat)
+            (e : A),
+        hbt = (HNode A h_hbt (Node A (Triple A hbt1 e hbt2))) ->
+        occ_hbt A compare x hbt =
+        match compare x e with
+        | Lt =>
+          occ_hbt A compare x hbt1
+        | Eq =>
+          true
+        | Gt =>
+          occ_hbt A compare x hbt2
+        end).
 
-Definition specification_of_occurs_bt
-           (A : Type)
-           (compare : A -> A -> element_comparison)
-           (occ_bt : forall (A' : Type),
-               (A' -> A' -> element_comparison)
-               -> A'
-               -> binary_tree A'
-               -> bool) :=
-  (forall (e : A),
-      occ_bt A compare e (Leaf A) = false)
-  /\
-  (forall (e : A)
-          (t : triple A),
-      exists (occ_t : forall (A' : Type),
-                 (A' -> A' -> element_comparison) -> A' -> triple A' -> bool),
-        occ_bt A compare e (Node A t) = occ_t A compare e t).
-
-Definition specification_of_occurs_t
-           (A : Type)
-           (compare : A -> A -> element_comparison)
-           (occ_t : forall (A' : Type),
-               (A' -> A' -> element_comparison)
-               -> A'
-               -> triple A'
-               -> bool) :=
-  forall (e e' : A)
-         (hbt1 hbt2 : heightened_binary_tree A),
-    exists (occ_hbt : forall (A' : Type),
-               (A' -> A' -> element_comparison)
-               -> A'
-               -> heightened_binary_tree A'
-               -> bool),
-      occ_t A compare e (Triple A hbt1 e' hbt2) =
-      match compare e e' with
-      | Lt =>
-        occ_hbt A compare e hbt1
-      | Eq =>
-        true
-      | Gt =>
-        occ_hbt A compare e hbt2
-      end.
-                
-    
-
-(* Theorem to show that occurs_hbt, occurs_bt, and occurs_t meet their respective  *)
-(*  * specifications *)
+(** Theorem to show that our implementation of lookup on AVL trees, [occurs_hbt], 
+meets the [specification_of_occurs_hbt] *)
 Theorem occurs_implementation_satisfies_its_specification:
   forall (A : Type)
          (compare : A -> A -> element_comparison),
-  (specification_of_occurs_hbt A compare occurs_hbt)
-  /\
-  (specification_of_occurs_bt A compare occurs_bt)
-  /\
-  (specification_of_occurs_t A compare occurs_t).
+    specification_of_occurs_hbt A compare occurs_hbt.
 Proof.
-  intros A compare.
-  split.
+  intros.
+  unfold specification_of_occurs_hbt.
+  intros.
+  split. 
 
-  - unfold specification_of_occurs_hbt.
-    intros e h bt.
-    exists occurs_bt.
+  (* hbt is a leaf *)
+  - intro.
+    rewrite -> H0.
+    rewrite -> unfold_occurs_hbt.
+    rewrite -> unfold_occurs_bt_leaf.
     reflexivity.
 
-  - split.
-    unfold specification_of_occurs_bt.
-    split.
-    intro e.
-    rewrite -> (unfold_occurs_bt_leaf A compare e).
-    reflexivity.
-    intros e t.
-    exists occurs_t.
-    Check (unfold_occurs_bt_node).
-    rewrite -> (unfold_occurs_bt_node A compare e t).
-    reflexivity.
-
-    unfold specification_of_occurs_t.
-    intros e e' hbt1 hbt2.
-    exists occurs_hbt.
-    Check (unfold_occurs_t).
-    rewrite -> (unfold_occurs_t A compare e e' hbt1 hbt2).
+  (* hbt is a node *)  
+  - intros.
+    rewrite -> H0.
+    rewrite -> unfold_occurs_hbt.
+    rewrite -> unfold_occurs_bt_node.
+    rewrite -> unfold_occurs_t.
     reflexivity.
 Qed.
 
-(* ***** Section 2: The specifications and theorems for insert  ***** *)
+(* ********** *)
 
+(* ********** *)
+
+(** * Insertion *)
+
+(** Defining the specification for an insertion function on AVL trees: given a sound,
+balanced, and ordered tree, inserting some element into this tree should give a tree 
+that is also sound, balanced, and ordered *)
 Definition specifiction_of_insert_hbt
            (A : Type)
            (compare : A -> A -> element_comparison)
@@ -125,6 +97,8 @@ Definition specifiction_of_insert_hbt
     /\
     (is_ordered_hbt A (insert_hbt A compare x hbt) compare = true).
   
+(** Theorem to show that our implementation of insertion on AVL trees, 
+[insert_hbt] meets the [specifiction_of_insert_hbt] *)
 Theorem insert_hbt_satisfies_its_specification:
   forall (A : Type)
          (compare : A -> A -> element_comparison)
@@ -137,8 +111,7 @@ Proof.
   unfold insert_hbt.
   case (insert_hbt_helper A compare x hbt) as [ hbt' | ] eqn : C.
 
-  - Check (insertion_preserves_soundness).
-    destruct (insertion_preserves_soundness A compare x) as
+  - destruct (insertion_preserves_soundness A compare x) as
         [H_hbt_sound _].
     split.
 
@@ -149,8 +122,6 @@ Proof.
       split.
       exact (H_hbt_balance hbt hbt' H_sound_init H_bal_init C).
 
-      
-      Check (insertion_preserves_order).
       destruct (insertion_preserves_order A compare x H_compare) as [H_ord _].
       exact (H_ord hbt hbt' H_sound_init H_bal_init H_order_init C).
 
@@ -162,3 +133,7 @@ Proof.
 
     exact H_order_init.
 Qed.
+
+(* ********** *)
+
+(* ********** End of theorems.v ********** *)
